refactor

theories/LambdaCalculus/Reductions/KrivineMclosed_HALT_to_MMA_HALTING.v
@@ -1,6 +1,8 @@
 (* TODO move to MinskyMachines *)
 From Undecidability Require Import
   LambdaCalculus.Krivine MinskyMachines.MM.
+From Undecidability Require Import
+  LambdaCalculus.Util.Krivine_facts.
 From Undecidability Require
   LambdaCalculus.Krivine MinskyMachines.MMA.mma_defs.
 From Undecidability.Shared.Libs.DLW
@@ -12,13 +14,14 @@ Require Import ssreflect ssrbool ssrfun.
 
 Import L (term, var, app, lam).
 
+#[local] Unset Implicit Arguments.
+
 #[local] Notation mm_instr := (mm_instr (pos 5)).
 #[local] Notation counter := (pos 5).
 #[local] Notation mm_state := (mm_state 5).
 
-#[local] Notation "P // s -[ k ]-> t" := (sss_steps (@mma_sss _) P k s t).
-#[local] Notation "P // s ->> t" := (sss_compute (@mma_sss _) P s t).
-#[local] Notation "P // s -+> t" := (sss_progress (@mma_sss _) P s t).
+#[local] Notation "P // s ->> t" := (sss_compute (@mma_sss 5) P s t).
+#[local] Notation "P // s -+> t" := (sss_progress (@mma_sss 5) P s t).
 #[local] Notation "e #> x" := (vec_pos e x).
 #[local] Notation "e [ v / x ]" := (vec_change e x v).
 
@@ -76,11 +79,12 @@ Proof. exists 0. by apply: in_sss_steps_0. Qed.
 Fact sss_compute_refl' i P (st1 st2 : mm_state) : st1 = st2 -> (i, P) // st1 ->> st2.
 Proof. move=> ->. by apply: sss_compute_refl. Qed.
 
-(* X := 0 *)
-Definition ZERO (X: counter) (offset: nat) : list mm_instr :=
-  [DEC X (0+offset)].
-
-Definition ZERO_len := 1.
+Lemma sss_compute_progress P st st' : P // st ->> st' -> st <> st' -> P // st -+> st'.
+Proof.
+  move=> [[|k]].
+  - by move=> /sss_steps_0_inv.
+  - move=> Hk _. exists (S k). by split; [lia|].
+Qed.
 
 Lemma mma_step {P : list mm_instr} {offset} i {v st} : 
   match nth_error P i with
@@ -113,6 +117,45 @@ Proof.
       split; [done|]. by apply: in_mma_sss_dec_1.
 Qed.
 
+(* uses uniform subproc contac structure *)
+Lemma concat_sss_compute_trans {Ps : list (list mm_instr)} {offset} (i : nat) {v st st'} :
+  let j := length (concat (firstn i Ps)) in
+  (j + offset, nth i Ps []) // (j + offset, v) ->> st' ->
+  (offset, concat Ps) // st' ->> st ->
+  (offset, concat Ps) // (j + offset, v) ->> st.
+Proof.
+  move=> j H. apply: sss_compute_trans.
+  have : ({(j + offset, v) = st'} + {(j + offset, v) <> st'}).
+  { do ? decide equality. apply: vec_eq_dec. by apply: Nat.eq_dec. }
+  move=> [<-|H']. { by apply: sss_compute_refl. }
+  apply: (subcode_sss_compute (P := (_, nth i Ps []))).
+  - exists (concat (firstn i Ps)), (concat (skipn (S i) Ps)).
+    split; last done.
+    have -> : nth i Ps [] = concat [nth i Ps []].
+    { by rewrite /concat app_nil_r. }
+    rewrite -?concat_app. congr concat.
+    rewrite [LHS](esym (firstn_skipn i Ps)). congr List.app.
+    have : nth i Ps [] <> [].
+    { move=> H''. move: H. rewrite H''.
+      move=> [[|k]].
+      - by move=> /sss_steps_0_inv.
+      - move=> /sss_steps_S_inv' [?] [+ _].
+        by move=> [?] [[|??]] [?] [?] [?] [[]]. }
+    elim: (i) (Ps); first by case.
+    move=> i' IH [|? ?]; first done.
+    rewrite !skipn_cons. by apply: IH.
+  - by rewrite (Nat.add_comm offset).
+Qed.
+
+#[local] Arguments plus : simpl never.
+#[local] Arguments concat : simpl never.
+
+(* X := 0 *)
+Definition ZERO (X: counter) (offset: nat) : list mm_instr :=
+  [DEC X (0+offset)].
+
+Definition ZERO_len := 1.
+
 Lemma ZERO_spec X v offset :
   (offset, ZERO X offset) // (0 + offset, v) ->> (ZERO_len+offset, vec_change v X 0).
 Proof.
@@ -139,11 +182,11 @@ Proof.
   by apply: sss_compute_refl.
 Qed.
 
-Arguments plus : simpl never.
-
 (* Y := X + Y *)
 Definition MOVE (X Y: counter) (offset: nat) : list mm_instr :=
-  JMP (3+offset) ++ [INC Y; DEC X (2+offset)].
+  concat (
+    JMP (3+offset) ::
+    [INC Y; DEC X (2+offset)] :: []).
 
 Definition MOVE_len := length (MOVE A A 0).
 
@@ -154,10 +197,7 @@ Lemma MOVE_spec X Y v offset :
   (offset, MOVE X Y offset) // (offset, v) ->> (MOVE_len+offset, vec_change (vec_change v Y (y+x)) X 0).
 Proof.
   move=> /= HXY.
-  apply: sss_compute_trans.
-  { apply: (subcode_sss_compute (P := (_, JMP _))).
-    { by eexists [], _. }
-    rewrite /= Nat.add_0_r. by apply: JMP_spec. }
+  apply: (concat_sss_compute_trans 0). { by apply: JMP_spec. }
   move En: (vec_pos v X) => n.
   move Ew: (vec_change _ X 0) => w.
   elim: n v En w Ew.
@@ -168,15 +208,16 @@ Proof.
     apply: mma_step. rewrite /= En.
     apply: mma_step. apply: IH.
     + by rewrite !(vec_norm HXY).
-    + rewrite !(vec_norm HXY). congr vec_change. congr vec_change. lia.
+    + rewrite !(vec_norm HXY). do ? congr vec_change. lia.
 Qed.
 
 (* Y := X *)
 Definition COPY (X Y: counter) (offset: nat) : list mm_instr :=
-  let i := offset in JMP (2+JMP_len+i) ++
-  let j := JMP_len + i in [INC A; INC Y] ++
-  let i := 2 + j in [DEC X j] ++
-  let i := 1 + i in MOVE A X i ++ [].
+  concat ( 
+    let i := offset in JMP (2+JMP_len+i) ::
+    let j := JMP_len + i in [INC A; INC Y] ::
+    let i := 2 + j in [DEC X j] ::
+    let i := 1 + i in MOVE A X i :: []).
 
 Definition COPY_len := length (COPY A A 0).
 
@@ -186,35 +227,29 @@ Lemma COPY_spec X Y v offset :
   (offset, COPY X Y offset) // (offset, v) ->>
     (COPY_len+offset, vec_change (vec_change (vec_change v X (a+x)) Y (x+y)) A 0).
 Proof.
-  move=> /= HX HY HXY. have H' : forall i, offset + i = i + offset by lia.
-  apply: sss_compute_trans.
-  { apply: (subcode_sss_compute (P := (_, JMP _))).
-    { by eexists [], _. }
-    rewrite ?H'. by apply: JMP_spec. }
+  move=> /= HX HY HXY.
+  apply: (concat_sss_compute_trans 0). { by apply: JMP_spec. }
   move Ew: (vec_change _ A _) => w.
   elim /(measure_ind (fun v => vec_pos v X)): v w Ew.
   move=> v IH w <-. case Ex: (vec_pos v X) => [|x].
   { apply: mma_step. rewrite /= Ex.
-    apply: sss_compute_trans.
-    { apply: (subcode_sss_compute (P := (_, MOVE _ _ _))).
-      { eexists _, _. rewrite /COPY. by do 2 rewrite [LHS]app_assoc. }
-      rewrite ?H'. by apply: MOVE_spec. }
+    apply: (concat_sss_compute_trans 3). { by apply: MOVE_spec. }
     apply: sss_compute_refl'. congr pair.
-    congr vec_change. rewrite !(vec_norm HXY). congr vec_change. lia. }
+    rewrite !(vec_norm HXY). do ? congr vec_change. lia. }
   apply: mma_step. rewrite /= Ex.
   apply: mma_step. apply: mma_step. apply: IH.
   - rewrite !(vec_norm HXY) !(vec_norm HX). lia.
   - do ? rewrite ?(vec_norm HX) ?(vec_norm HY) ?(vec_norm HXY).
-    congr vec_change. congr vec_change; last by lia.
-    congr vec_change. lia.
+    do ? congr vec_change; lia.
 Qed.
 
 (* X := X+X *)
 Definition DOUBLE (X: counter) (offset: nat) : list mm_instr :=
-  let i := offset in ZERO A offset ++ 
-  let i := ZERO_len + i in JMP (JMP_len + 2 + i) ++
-  let i := JMP_len + i in [INC A; INC A; DEC X i] ++
-  let i := 3 + i in MOVE A X i.
+  concat (
+    let i := offset in ZERO A offset ::
+    let i := ZERO_len + i in JMP (JMP_len + 2 + i) ::
+    let i := JMP_len + i in [INC A; INC A; DEC X i] ::
+    let i := 3 + i in MOVE A X i :: []).
 
 Definition DOUBLE_len := length (DOUBLE A 0).
 
@@ -226,16 +261,9 @@ Lemma DOUBLE_spec X v offset :
   (offset, DOUBLE X offset) // (offset, v) ->>
     (DOUBLE_len+offset, vec_change (vec_change v X (x+x)) A 0).
 Proof.
-  have H' : forall i, offset + i = i + offset by lia.
   move=> /= HX.
-  apply: sss_compute_trans.
-  { apply: (subcode_sss_compute (P := (offset, ZERO A offset))).
-    { exists []. eexists. split; [done|rewrite /=; lia]. }
-    by apply: ZERO_spec. }
-  apply: sss_compute_trans.
-  { apply: (subcode_sss_compute (P := (_, JMP _))).
-    { rewrite /= /DOUBLE. by do 2 eexists. }
-    rewrite ?H'. by apply: JMP_spec. }
+  apply: (concat_sss_compute_trans 0). { by apply: ZERO_spec. }
+  apply: (concat_sss_compute_trans 1). { by apply: JMP_spec. }
   move Ev': (vec_change v A 0) => v'.
   have :
     let x := vec_pos v' X in forall w, w = vec_change (vec_change v' X 0) A (x+x+(vec_pos v' A)) ->
@@ -255,21 +283,19 @@ Proof.
       + by rewrite !(vec_change_neq HX) vec_change_eq.
       + rewrite !(vec_norm HX). congr vec_change. lia. }
   move=> /(_ _ erefl) /sss_compute_trans. apply.
-  apply: sss_compute_trans.
-  { apply: (subcode_sss_compute (P := (_, MOVE _ _ _))).
-    { rewrite /= /DOUBLE. do 2 eexists. by do 2 rewrite [LHS]app_assoc. }
-      rewrite ?H'. by apply: MOVE_spec. }
+  apply: (concat_sss_compute_trans 3). { by apply: MOVE_spec. }
   apply: sss_compute_refl'. congr pair.
-  rewrite -Ev' !(vec_norm HX). congr vec_change. congr vec_change. lia.
+  rewrite -Ev' !(vec_norm HX). do ? congr vec_change. lia.
 Qed.
 
 (* X := (X+X+1)*(2^Y) *)
 Definition PACK (X Y: counter) (offset: nat) : list mm_instr :=
-  DOUBLE X offset ++
-  let i := DOUBLE_len + offset in [INC X] ++
-  let i := 1 + i in JMP (DOUBLE_len+JMP_len+i) ++
-  let i := JMP_len + i in DOUBLE X i ++
-  [DEC Y i].
+  concat (
+    DOUBLE X offset ::
+    let i := DOUBLE_len + offset in [INC X] ::
+    let i := 1 + i in JMP (DOUBLE_len+JMP_len+i) ::
+    let i := JMP_len + i in DOUBLE X i ::
+    [DEC Y i] :: []).
 
 Definition PACK_len := length (PACK A A 0).
 
@@ -280,16 +306,10 @@ Lemma PACK_spec X Y v offset :
   (offset, PACK X Y offset) // (offset, v) ->>
     (PACK_len+offset, vec_change (vec_change (vec_change v X ((x+x+1) * (2 ^ y))) Y 0) A 0).
 Proof.
-  move=> /= HX HY HXY. have H' : forall i, offset + i = i + offset by lia.
-  apply: sss_compute_trans.
-  { apply: (subcode_sss_compute (P := (_, DOUBLE _ _))).
-    { exists []. by eexists. }
-    rewrite ?H'. by apply: DOUBLE_spec. }
+  move=> /= HX HY HXY.
+  apply: (concat_sss_compute_trans 0). { by apply: DOUBLE_spec. }
   apply: mma_step.
-  apply: sss_compute_trans.
-  { apply: (subcode_sss_compute (P := (_, JMP _))).
-    { do 2 eexists. rewrite /PACK. by rewrite [LHS]app_assoc. }
-    rewrite ?H'. by apply: JMP_spec. }
+  apply: (concat_sss_compute_trans 2). { by apply: JMP_spec. }
   move Ev': (v' in _ // (_, v') ->> _) => v'.
   have HAv' : vec_pos v' A = 0.
   { by rewrite -Ev' (vec_change_neq (nesym HX)) vec_change_eq. }
@@ -308,10 +328,7 @@ Proof.
       lia.
     - move=> n IH v'' En HAv'' w ->.
       rewrite !Nat.add_assoc. apply: mma_step. rewrite /= En.
-      apply: sss_compute_trans.
-      { apply: (subcode_sss_compute (P := (_, DOUBLE _ _))).
-        { do 2 eexists. rewrite /PACK. by do 2 rewrite app_assoc. }
-        rewrite ?H'. by apply: DOUBLE_spec. }
+      apply: (concat_sss_compute_trans 3). { by apply: DOUBLE_spec. }
       apply: IH.
       + by rewrite !(vec_change_neq HY) !(vec_change_neq HXY) vec_change_eq.
       + by rewrite vec_change_eq.
@@ -325,13 +342,14 @@ Qed.
 
 (* X := X/2 + A if X even goto p else goto q *)
 Definition HALF (X: counter) (p q: nat) (offset: nat) : list mm_instr :=
-  let i := offset in JMP (JMP_len + 1 + i) ++
-  let i := JMP_len + i in let j := i in [INC A; DEC X (2+JMP_len+MOVE_len+i)] ++
-  let i := 2 + i in MOVE A X i ++
-  let i := MOVE_len + i in JMP p ++
-  let i := JMP_len + i in [DEC X j] ++
-  let i := 1 + i in MOVE A X i ++
-  let i := MOVE_len + i in JMP q ++ [].
+  concat (
+    let i := offset in JMP (JMP_len + 1 + i) ::
+    let i := JMP_len + i in let j := i in [INC A; DEC X (2+JMP_len+MOVE_len+i)] ::
+    let i := 2 + i in MOVE A X i ::
+    let i := MOVE_len + i in JMP p ::
+    let i := JMP_len + i in [DEC X j] ::
+    let i := 1 + i in MOVE A X i ::
+    let i := MOVE_len + i in JMP q :: []).
 
 Definition HALF_len := length (HALF A 0 0 0).
 
@@ -367,51 +385,37 @@ Lemma HALF_spec X p q v offset :
   (offset, HALF X p q offset) // (offset, v) ->>
     let '(m, b) := half x in (if b then p else q, vec_change (vec_change v X (a+m)) A 0).
 Proof.
-  move=> /= HX. have H' : forall i, offset + i = i + offset by lia.
-  apply: sss_compute_trans.
-  { apply: (subcode_sss_compute (P := (_, JMP _))).
-    { by eexists [], _. }
-    rewrite ?H'. by apply: JMP_spec. }
+  move=> /= HX.
+  apply: (concat_sss_compute_trans 0). { by apply: JMP_spec. }
   move Hst: (st in _ // _ ->> st) => st.
   elim /(measure_ind (fun v => vec_pos v X)) : v st Hst.
   move=> v IH st <-.
   case EX: (vec_pos v X) => [|[|n]].
   { apply: mma_step. rewrite /= EX.
-    apply: sss_compute_trans.
-    { apply: (subcode_sss_compute (P := (_, MOVE _ _ _))).
-      { eexists _, _. by rewrite /HALF [LHS]app_assoc. }
-      rewrite ?H'. by apply: MOVE_spec. }
-    apply: sss_compute_trans.
-    { apply: (subcode_sss_compute (P := (_, JMP _))).
-      { eexists _, _. by rewrite /HALF [LHS]app_assoc [LHS]app_assoc. }
-      rewrite ?H'. by apply: JMP_spec. }
+    apply: (concat_sss_compute_trans 2). { by apply: MOVE_spec. }
+    apply: (concat_sss_compute_trans 3). { by apply: JMP_spec. }
     apply: sss_compute_refl'. by rewrite EX !Nat.add_0_r. }
   { apply: mma_step. rewrite /= EX !Nat.add_assoc.
     apply: mma_step. rewrite /= (vec_change_eq erefl).
-    apply: sss_compute_trans.
-    { apply: (subcode_sss_compute (P := (_, MOVE _ _ _))).
-      { eexists _, _. rewrite /HALF. by do 4 rewrite [LHS]app_assoc. }
-      rewrite ?H'. by apply: MOVE_spec. }
-    apply: sss_compute_trans.
-    { apply: (subcode_sss_compute (P := (_, JMP _))).
-      { eexists _, _. rewrite /HALF. by do 5 rewrite [LHS]app_assoc. }
-      rewrite ?H'. by apply: JMP_spec. }
+    apply: (concat_sss_compute_trans 5). { by apply: MOVE_spec. }
+    apply: (concat_sss_compute_trans 6). { by apply: JMP_spec. }
     apply: sss_compute_refl'. by rewrite !(vec_norm HX) !Nat.add_0_r. }
   apply: mma_step. rewrite /= EX !Nat.add_assoc.
   apply: mma_step. rewrite /= (vec_change_eq erefl).
   apply: mma_step. apply: IH. { rewrite !(vec_norm HX). lia. }
   rewrite !(vec_norm HX) /=.
   have := half_spec n. case: (half n) => m [] ->.
-  - rewrite !(vec_norm HX). congr pair. congr vec_change. congr vec_change. lia.
-  - rewrite !(vec_norm HX). congr pair. congr vec_change. congr vec_change. lia.
+  - rewrite !(vec_norm HX). congr pair. do ? congr vec_change. lia.
+  - rewrite !(vec_norm HX). congr pair. do ? congr vec_change. lia.
 Qed.
 
 (* IF X = 0 then GOTO p else GOTO q *)
 Definition BR (X: counter) (p q: nat) (offset: nat) : list mm_instr :=
-  let i := offset in [DEC X (JMP_len + 1 + i)] ++
-  let i := 1 + i in JMP p ++
-  let i := JMP_len + i in [INC X] ++
-  let i := 1 + i in JMP q ++ [].  
+  concat (
+    let i := offset in [DEC X (JMP_len + 1 + i)] ::
+    let i := 1 + i in JMP p ::
+    let i := JMP_len + i in [INC X] ::
+    let i := 1 + i in JMP q :: []).  
 
 Definition BR_len := length (BR A 0 0 0).
 
@@ -419,31 +423,26 @@ Lemma BR_spec X p q v offset :
   let x := vec_pos v X in
   (offset, BR X p q offset) // (offset, v) ->> (if x is 0 then p else q, v).
 Proof.
-  move=> /=. have H' : forall i, offset + i = i + offset by lia.
+  move=> /=.
   case EX: (vec_pos v X) => [|n].
   - apply: (mma_step 0). rewrite /= EX.
-    apply: sss_compute_trans.
-    { apply: (subcode_sss_compute (P := (_, JMP _))).
-      { eexists _, _. done. }
-      rewrite ?H'. by apply: JMP_spec. }
-    by apply: sss_compute_refl'.
+    apply: (concat_sss_compute_trans 1). { by apply: JMP_spec. }
+    by apply: sss_compute_refl.
   - apply: (mma_step 0). rewrite /= EX. apply: mma_step.
-    apply: sss_compute_trans.
-    { apply: (subcode_sss_compute (P := (_, JMP _))).
-      { eexists _, _. rewrite /BR. by do 2 rewrite [LHS]app_assoc. }
-      rewrite ?H'. by apply: JMP_spec. }
-    apply: sss_compute_refl'. congr pair.
+    apply: (concat_sss_compute_trans 3). { by apply: JMP_spec. }
+    apply: sss_compute_refl'.
     by rewrite (vec_change_eq erefl) vec_change_idem -EX vec_change_same.
 Qed.
 
 (* IF X = (n+n+1)*2^m THEN X := n AND Y := m *)
 Definition UNPACK (X Y: counter) (offset: nat) : list mm_instr :=
-  let i := offset in BR X 0 (BR_len + i) i ++
-  let i := BR_len + i in ZERO A i ++
-  let i := ZERO_len + i in ZERO Y i ++
-  let j := ZERO_len + i in HALF X (HALF_len + j) (JMP_len + 1 + HALF_len + j) j ++
-  let i := HALF_len + j in [INC Y] ++
-  let i := 1 + i in JMP j ++ [].
+  concat (
+    let i := offset in BR X 0 (BR_len + i) i ::
+    let i := BR_len + i in ZERO A i ::
+    let i := ZERO_len + i in ZERO Y i ::
+    let j := ZERO_len + i in HALF X (HALF_len + j) (JMP_len + 1 + HALF_len + j) j ::
+    let i := HALF_len + j in [INC Y] ::
+    let i := 1 + i in JMP j :: []).
 
 Definition UNPACK_len := length (UNPACK A A 0).
 
@@ -454,21 +453,12 @@ Lemma UNPACK_spec {X Y m n v offset} :
   (offset, UNPACK X Y offset) // (offset, v) ->>
     (UNPACK_len + offset, vec_change (vec_change (vec_change v X n) Y m) A 0).
 Proof.
-  move=> /= H'X HX HY HXY. have H' : forall i, offset + i = i + offset by lia.
-  apply: sss_compute_trans.
-  { apply: (subcode_sss_compute (P := (_, BR _ _ _ _))).
-    { by eexists [], _. }
-    rewrite ?H'. by apply: BR_spec. }
+  move=> /= H'X HX HY HXY.
+  apply: (concat_sss_compute_trans 0). { by apply: BR_spec. }
   have ->: vec_pos v X = S (vec_pos v X - 1).
   { rewrite H'X. have := Nat.pow_nonzero 2 m. lia. }
-  apply: sss_compute_trans.
-  { apply: (subcode_sss_compute (P := (_, ZERO _ _))).
-    { by eexists _, _. }
-    rewrite ?H'. by apply: ZERO_spec. }
-  apply: sss_compute_trans.
-  { apply: (subcode_sss_compute (P := (_, ZERO _ _))).
-    { eexists _, _. by rewrite /UNPACK [LHS]app_assoc. }
-    rewrite ?H'. by apply: ZERO_spec. }
+  apply: (concat_sss_compute_trans 1). { by apply: ZERO_spec. }
+  apply: (concat_sss_compute_trans 2). { by apply: ZERO_spec. }
   suff : forall v' w', 
     w' = vec_change (vec_change v' X n) Y (m + vec_pos v' Y) ->
     vec_pos v' X = (n + n + 1) * 2 ^ m ->
@@ -481,24 +471,15 @@ Proof.
     - by rewrite !(vec_norm HY). }
   elim: m {H'X}.
   { move=> v' w' -> H'v' H''v'.
-    apply: sss_compute_trans.
-    { apply: (subcode_sss_compute (P := (_, HALF _ _ _ _))).
-      { eexists _, _. rewrite /UNPACK. by do 2 rewrite [LHS]app_assoc. }
-      rewrite ?H'. by apply: HALF_spec. }
+    apply: (concat_sss_compute_trans 3). { by apply: HALF_spec. }
     rewrite H'v' half_spec_odd.
     apply: sss_compute_refl'. congr pair.
     rewrite H''v' !Nat.add_0_l !(vec_norm HXY) !(vec_norm (nesym HX)).
     congr vec_change. by rewrite vec_change_same'. }
   move=> m IH v' w' -> H'v' H''v'.
-  apply: sss_compute_trans.
-  { apply: (subcode_sss_compute (P := (_, HALF _ _ _ _))).
-    { eexists _, _. rewrite /UNPACK. by do 2 rewrite [LHS]app_assoc. }
-    rewrite ?H'. by apply: HALF_spec. }
+  apply: (concat_sss_compute_trans 3). { by apply: HALF_spec. }
   rewrite H'v' half_spec_even !Nat.add_assoc. apply: mma_step.
-  apply: sss_compute_trans.
-  { apply: (subcode_sss_compute (P := (_, JMP _))).
-    { eexists _, _. rewrite /UNPACK. by do 4 rewrite [LHS]app_assoc. }
-    rewrite ?H'. by apply: JMP_spec. }
+  apply: (concat_sss_compute_trans 5). { by apply: JMP_spec. }
   apply: IH.
   - do ? rewrite ?(vec_norm (nesym HY)) ?(vec_norm (nesym HX)) ?(vec_norm HXY).
     rewrite (vec_change_same' v' A 0 H''v').
@@ -511,11 +492,8 @@ Lemma UNPACK_spec' {X Y v offset} :
   vec_pos v X = 0 ->
   (offset, UNPACK X Y offset) // (offset, v) ->> (0, v).
 Proof.
-  move=> H'X. have H' : forall i, offset + i = i + offset by lia.
-  apply: sss_compute_trans.
-  { apply: (subcode_sss_compute (P := (_, BR _ _ _ _))).
-    { by eexists [], _. }
-    rewrite ?H'. by apply: BR_spec. }
+  move=> H'X.
+  apply: (concat_sss_compute_trans 0). { by apply: BR_spec. }
   rewrite H'X. by apply: sss_compute_refl.
 Qed.
 
@@ -554,9 +532,10 @@ Proof.
 Qed.
 
 Definition CASE_VAR0 (p: nat) (offset : nat) : list mm_instr :=
-  let i := offset in UNPACK CTX U i ++
-  let i := UNPACK_len + i in UNPACK U CTX i ++
-  let i := UNPACK_len + i in JMP p.
+  concat (
+    let i := offset in UNPACK CTX U i ::
+    let i := UNPACK_len + i in UNPACK U CTX i ::
+    let i := UNPACK_len + i in JMP p :: []).
 
 Definition CASE_VAR0_len := length (CASE_VAR0 0 0).
 
@@ -565,31 +544,20 @@ Lemma CASE_VAR0_spec ctx' t' ctx p v offset :
   (offset, CASE_VAR0 p offset) // (offset, v) ->>
     (p, vec_change (vec_change (vec_change v U (enc_term t')) CTX (enc_cs ctx')) A 0).
 Proof.
-  move=> /= Hv. have H' : forall i, offset + i = i + offset by lia.
-  apply: sss_compute_trans.
-  { apply: (subcode_sss_compute (P := (_, UNPACK _ _ _))).
-    { by eexists [], _. }
-    rewrite ?H'. by apply: (UNPACK_spec Hv). }
-  move Ev': (vec_change _ A 0) => v'.
-  apply: sss_compute_trans.
-  { apply: (subcode_sss_compute (P := (_, UNPACK _ _ _))).
-    { by eexists _, _. }
-    rewrite ?H'.
-    have /= /UNPACK_spec : vec_pos v' U = enc_closure (closure ctx' t').
-    { by rewrite -Ev' (counters_eta v). } by apply. }
-  apply: sss_compute_trans.
-  { apply: (subcode_sss_compute (P := (_, JMP _))).
-    { eexists _, _. by rewrite /CASE_VAR0 [LHS]app_assoc. }
-    rewrite ?H'. by apply: JMP_spec. }
-  apply: sss_compute_refl'. congr pair.
-  by rewrite -Ev' (counters_eta v).
+  move=> /= Hv.
+  apply: (concat_sss_compute_trans 0). { by apply: (UNPACK_spec Hv). }
+  apply: (concat_sss_compute_trans 1).
+  { by apply: UNPACK_spec; first rewrite (counters_eta v). }
+  apply: (concat_sss_compute_trans 2). { by apply: JMP_spec. }
+  apply: sss_compute_refl'. by rewrite (counters_eta v).
 Qed.
 
 Definition CASE_VARS (p: nat) (offset : nat) : list mm_instr :=
-  let i := offset in UNPACK CTX B i ++
-  let i := UNPACK_len + i in ZERO B i ++
-  let i := ZERO_len + i in PACK U B i ++
-  let i := PACK_len + i in JMP p ++ [].
+  concat (
+    let i := offset in UNPACK CTX B i ::
+    let i := UNPACK_len + i in ZERO B i ::
+    let i := ZERO_len + i in PACK U B i ::
+    let i := PACK_len + i in JMP p :: []).
 
 Definition CASE_VARS_len := length (CASE_VARS 0 0).
 
@@ -600,35 +568,23 @@ Lemma CASE_VARS_spec u ctx n p v offset :
   (offset, CASE_VARS p offset) // (offset, v) ->>
     (p, vec_change (vec_change (vec_change v U (enc_term (var n))) CTX (enc_cs ctx)) A 0).
 Proof.
-  move=> /= HCTX HU HB. have H' : forall i, offset + i = i + offset by lia.
-  apply: sss_compute_trans.
-  { apply: (subcode_sss_compute (P := (_, UNPACK _ _ _))).
-    { by eexists [], _. }
-    rewrite ?H'. by apply: (UNPACK_spec HCTX). }
-  apply: sss_compute_trans.
-  { apply: (subcode_sss_compute (P := (_, ZERO _ _))).
-    { by eexists _, _. }
-    rewrite ?H'. by apply: ZERO_spec. }
-  apply: sss_compute_trans.
-  { apply: (subcode_sss_compute (P := (_, PACK _ _ _))).
-    { eexists _, _. by rewrite /CASE_VARS [LHS]app_assoc. }
-    rewrite ?H'. by apply: PACK_spec. }
-  apply: sss_compute_trans.
-  { apply: (subcode_sss_compute (P := (_, JMP _))).
-    { eexists _, _. rewrite /CASE_VARS. by do 2 rewrite [LHS]app_assoc. }
-    rewrite ?H'. by apply: JMP_spec. }
+  move=> /= HCTX HU HB.
+  apply: (concat_sss_compute_trans 0). { by apply: (UNPACK_spec HCTX). }
+  apply: (concat_sss_compute_trans 1). { by apply: ZERO_spec. }
+  apply: (concat_sss_compute_trans 2). { by apply: PACK_spec. }
+  apply: (concat_sss_compute_trans 3). { by apply: JMP_spec. }
   apply: sss_compute_refl'. move: HCTX HU HB. rewrite (counters_eta v) /=.
   by move=> ? -> ->.
 Qed.
 
 Definition CASE_APP (p: nat) (offset : nat) : list mm_instr :=
-  let i := offset in PACK B CTX i ++
-  let i := PACK_len + i in PACK TS B i ++
-  let i := PACK_len + i in COPY TS CTX i ++
-  let i := COPY_len + i in UNPACK CTX B i ++
-  let i := UNPACK_len + i in UNPACK B CTX i ++
-  let i := UNPACK_len + i in JMP p ++
-  [].
+  concat (
+    let i := offset in PACK B CTX i ::
+    let i := PACK_len + i in PACK TS B i ::
+    let i := PACK_len + i in COPY TS CTX i ::
+    let i := COPY_len + i in UNPACK CTX B i ::
+    let i := UNPACK_len + i in UNPACK B CTX i ::
+    let i := UNPACK_len + i in JMP p :: []).
 
 Definition CASE_APP_len := length (CASE_APP 0 0).
 
@@ -641,45 +597,29 @@ Lemma CASE_APP_spec ts ctx t p v offset :
   (offset, CASE_APP p offset) // (offset, v) ->>
     (p, vec_change (vec_change v TS (enc_cs ((closure ctx t)::ts))) A 0).
 Proof.
-  move=> /= HTS HCTX HB. have H' : forall i, offset + i = i + offset by lia.
-  apply: sss_compute_trans.
-  { apply: (subcode_sss_compute (P := (_, PACK _ _ _))).
-    { by eexists [], _. }
-    rewrite ?H'. by apply: PACK_spec. }
-  apply: sss_compute_trans.
-  { apply: (subcode_sss_compute (P := (_, PACK _ _ _))).
-    { by eexists _, _. }
-    rewrite ?H'. by apply: PACK_spec. }
-  apply: sss_compute_trans.
-  { apply: (subcode_sss_compute (P := (_, COPY _ _ _))).
-    { eexists _, _. rewrite /CASE_APP. by do 1 rewrite [LHS]app_assoc. }
-    rewrite ?H'. by apply: COPY_spec. }
+  move=> /= HTS HCTX HB.
+  apply: (concat_sss_compute_trans 0). { by apply: PACK_spec. }
+  apply: (concat_sss_compute_trans 1). { by apply: PACK_spec. }
+  apply: (concat_sss_compute_trans 2). { by apply: COPY_spec. }
   do ? (rewrite ?(vec_change_eq erefl); try (rewrite vec_change_neq; first done)).
-  apply: sss_compute_trans.
-  { apply: (subcode_sss_compute (P := (_, UNPACK _ _ _))).
-    { eexists _, _. rewrite /CASE_APP. by do 2 rewrite [LHS]app_assoc. }
-    rewrite ?H'. apply: UNPACK_spec; [|done ..].
+  apply: (concat_sss_compute_trans 3). 
+  { apply: UNPACK_spec; [|done ..].
     do ? (rewrite ?(vec_change_eq erefl); try (rewrite vec_change_neq; first done)).
     by rewrite Nat.add_0_r. }
-  apply: sss_compute_trans.
-  { apply: (subcode_sss_compute (P := (_, UNPACK _ _ _))).
-    { eexists _, _. rewrite /CASE_APP. by do 3 rewrite [LHS]app_assoc. }
-    rewrite ?H'. apply: UNPACK_spec; [|done ..].
+  apply: (concat_sss_compute_trans 4). 
+  { apply: UNPACK_spec; [|done ..].
     do ? (rewrite ?(vec_change_eq erefl); try (rewrite vec_change_neq; first done)).
     done. }
-  apply: sss_compute_trans.
-  { apply: (subcode_sss_compute (P := (_, JMP _))).
-    { eexists _, _. rewrite /CASE_APP. by do 4 rewrite [LHS]app_assoc. }
-    rewrite ?H'. by apply: JMP_spec. }
+  apply: (concat_sss_compute_trans 5). { by apply: JMP_spec. }
   apply: sss_compute_refl'. move: HTS HCTX HB. rewrite (counters_eta v) /=.
   by move=> -> -> ->.
 Qed.
 
 Definition CASE_LAM (p: nat) (offset : nat) : list mm_instr :=
-  let i := offset in UNPACK TS B i ++
-  let i := UNPACK_len + i in PACK CTX B i ++
-  let i := PACK_len + i in JMP p ++
-  [].
+  concat (
+    let i := offset in UNPACK TS B i ::
+    let i := UNPACK_len + i in PACK CTX B i ::
+    let i := PACK_len + i in JMP p :: []).
 
 Definition CASE_LAM_len := length (CASE_LAM 0 0).
 
@@ -690,19 +630,10 @@ Lemma CASE_LAM_spec t ts ctx p v offset :
   (offset, CASE_LAM p offset) // (offset, v) ->>
     (p, vec_change (vec_change (vec_change v TS (enc_cs ts)) CTX (enc_cs (t::ctx))) A 0).
 Proof.
-  move=> /= HTS HCTX HB. have H' : forall i, offset + i = i + offset by lia.
-  apply: sss_compute_trans.
-  { apply: (subcode_sss_compute (P := (_, UNPACK _ _ _))).
-    { by eexists [], _. }
-    rewrite ?H'. by apply: (UNPACK_spec HTS). }
-  apply: sss_compute_trans.
-  { apply: (subcode_sss_compute (P := (_, PACK _ _ _))).
-    { by eexists _, _. }
-    rewrite ?H'. by apply: PACK_spec. }
-  apply: sss_compute_trans.
-  { apply: (subcode_sss_compute (P := (_, JMP _))).
-    { eexists _, _. rewrite /CASE_VARS. by do 1 rewrite [LHS]app_assoc. }
-    rewrite ?H'. by apply: JMP_spec. }
+  move=> /= HTS HCTX HB.
+  apply: (concat_sss_compute_trans 0). { by apply: (UNPACK_spec HTS). }
+  apply: (concat_sss_compute_trans 1). { by apply: PACK_spec. }
+  apply: (concat_sss_compute_trans 2). { by apply: JMP_spec. }
   apply: sss_compute_refl'. move: HTS HCTX HB. rewrite (counters_eta v) /=.
   by move=> ? -> ->.
 Qed.
@@ -711,97 +642,22 @@ Lemma CASE_LAM_spec' p v offset :
   vec_pos v TS = enc_cs [] ->
   (offset, CASE_LAM p offset) // (offset, v) ->> (0, v).
 Proof.
-  move=> /= HTS. have H' : forall i, offset + i = i + offset by lia.
-  apply: sss_compute_trans.
-  { apply: (subcode_sss_compute (P := (_, UNPACK _ _ _))).
-    { by eexists [], _. }
-    rewrite ?H'. by apply: (UNPACK_spec' HTS). }
+  move=> /= HTS.
+  apply: (concat_sss_compute_trans 0). { by apply: (UNPACK_spec' HTS). }
   by apply: sss_compute_refl.
 Qed.
 
-Definition NOOP (offset : nat) : list mm_instr :=
-  JMP (JMP_len + offset).
-
-Definition NOOP_len := length (NOOP 0).
-
-Lemma NOOP_spec v offset :
-  (offset, NOOP offset) // (offset, v) -+> (NOOP_len+offset, v).
-Proof.
-  exists 2. split; first by lia.
-  apply: in_sss_steps_S. { 
-    eexists _, [], _, [_], _. split; first done.
-    rewrite /= Nat.add_0_r. split; first done.
-    by apply: in_mma_sss_inc. }
-  apply: in_sss_steps_S. { 
-    eexists _, [_], _, [], _. split; first done.
-    rewrite /= (Nat.add_comm offset). split; first done.
-    apply: in_mma_sss_dec_1. by rewrite vec_change_eq. }
-  rewrite vec_change_idem vec_change_same.
-  by apply: in_sss_steps_0.
-Qed.
-
 Definition PROG (offset : nat) : list mm_instr :=
-  let i := offset in NOOP i ++
-  let i := NOOP_len + i in UNPACK U B i ++
-  let i := UNPACK_len + i in [DEC B (CASE_VARS_len+CASE_VAR0_len+2+i)] ++
-  (* var _ CASE *) let i := 1 + i in [DEC U (CASE_VAR0_len+1+i)] ++
-  (* var 0 CASE *) let i := 1 + i in CASE_VAR0 offset i ++
-  (* var (S n) CASE *) let i := CASE_VAR0_len + i in CASE_VARS offset i ++
-  let i := CASE_VARS_len + i in [DEC B (CASE_LAM_len+1+i)] ++
-  (* lam s CASE *) let i := 1 + i in CASE_LAM offset i ++
-  (* app s t CASE *) let i := CASE_LAM_len + i in CASE_APP offset i ++
-  [].
-
-Definition Krivine_step : (list eterm * list eterm * term) -> option (list eterm * list eterm * term) :=
-  fun '(ts, ctx, t) =>
-  match t with
-  | var 0 => 
-      match ctx with
-      | [] => None
-      | (closure ctx t)::_ => Some (ts, ctx, t)
-      end
-  | var (S n) =>
-      match ctx with
-      | [] => None
-      | _::ctx => Some (ts, ctx, var n)
-      end
-  | lam s =>
-      match ts with
-      | [] => None
-      | t::ts => Some (ts, t::ctx, s)
-      end
-  | app s t => Some ((closure ctx t)::ts, ctx, s)
-  end.
-
-Lemma iter_plus {X} {f : X -> X} {x : X} n m : Nat.iter (n + m) f x = Nat.iter m f (Nat.iter n f x).
-Proof.
-  elim: m; first by rewrite Nat.add_0_r.
-  move=> m /= <-. by have ->: n + S m = S n + m by lia.
-Qed.
-
-Lemma oiter_None {X : Type} (f : X -> option X) k : Nat.iter k (obind f) None = None.
-Proof. elim: k; [done | by move=> /= ? ->]. Qed.
-
-Lemma Krivine_step_spec ts ctx t : halt_cbn ts ctx t <-> 
-  exists k ctx' t', Nat.iter k (obind Krivine_step) (Some (ts, ctx, t)) = Some ([], ctx', lam t').
-Proof.
-  split.
-  - elim.
-    1-4: by move=> > ? [n] [ctx'] [t'] IH; exists (S n), ctx', t'; rewrite (iter_plus 1 n).
-    move=> >. exists 0. by do 2 eexists.
-  - move=> [k] [ctx'] [t'].
-    elim: k ts ctx t. { move=> > [-> -> ->]. by apply: halt_lam. }
-    move=> k IH ts ctx t. rewrite (iter_plus 1 k) /=.
-    case: t.
-    + move=> [|n].
-      * case: ctx; first by rewrite oiter_None.
-        move=> [? ?] ? /IH ?. by apply: halt_var_0.
-      * case: ctx; first by rewrite oiter_None.
-        move=> [? ?] ? /IH ?. by apply: halt_var_S.
-    + move=> ?? /IH ?. by apply: halt_app.
-    + move=> ?. case: ts; first by rewrite oiter_None.
-      move=> ?? /IH ?. by apply: halt_lam_ts.
-Qed.
+  concat (
+    let i := offset in JMP (JMP_len + i) ::
+    let i := JMP_len + i in UNPACK U B i ::
+    let i := UNPACK_len + i in [DEC B (CASE_VARS_len+CASE_VAR0_len+2+i)] ::
+    (* var _ CASE *) let i := 1 + i in [DEC U (CASE_VAR0_len+1+i)] ::
+    (* var 0 CASE *) let i := 1 + i in CASE_VAR0 offset i ::
+    (* var (S n) CASE *) let i := CASE_VAR0_len + i in CASE_VARS offset i ::
+    let i := CASE_VARS_len + i in [DEC B (CASE_LAM_len+1+i)] ::
+    (* lam s CASE *) let i := 1 + i in CASE_LAM offset i ::
+    (* app s t CASE *) let i := CASE_LAM_len + i in CASE_APP offset i :: []).
 
 Lemma HAB : A <> B.
 Proof. done. Qed.
@@ -812,6 +668,7 @@ Proof. done. Qed.
 Lemma HBU : B <> U.
 Proof. done. Qed.
 
+(* PROG corresponds to Krivine_step *)
 Lemma PROG_spec ts ctx t v ts' ctx' t' offset :
   vec_pos v TS = enc_cs ts ->
   vec_pos v CTX = enc_cs ctx ->
@@ -823,7 +680,6 @@ Lemma PROG_spec ts ctx t v ts' ctx' t' offset :
     vec_pos w U = enc_term t' /\
     (offset, PROG offset) // (offset, v) -+> (offset, w).
 Proof.
-  have H' : forall i, offset + i = i + offset by lia.
   case: t.
   - move=> [|n] /=; (case: ctx; first done).
     + (* case (var 0) *)
@@ -833,20 +689,14 @@ Proof.
       split. { move: H2v. by rewrite (counters_eta v). }
       split. { move: H3v. by rewrite (counters_eta v). }
       apply: sss_progress_compute_trans.
-      { apply: (subcode_sss_progress (P := (_, NOOP _))).
-        { by eexists [], _. }
-        rewrite ?H'. by apply: NOOP_spec. }
-      apply: sss_compute_trans.
-      { apply: (subcode_sss_compute (P := (_, UNPACK _ _ _))).
-        { by eexists _, _. }
-        rewrite ?H'. by apply: (UNPACK_spec H3v). }
-      rewrite ?Nat.add_assoc. apply: mma_step. rewrite /= !(vec_norm HAB).
+      { apply: sss_compute_progress.
+        { by apply: (concat_sss_compute_trans 0); [apply JMP_spec | apply: sss_compute_refl]. }
+        case. rewrite /JMP_len /=. lia. }
+      apply: (concat_sss_compute_trans 1). { by apply: (UNPACK_spec H3v). }
+      rewrite /= ?Nat.add_assoc. apply: mma_step. rewrite /= !(vec_norm HAB).
       rewrite ?Nat.add_assoc. apply: mma_step. rewrite /= !(vec_norm HAU) !(vec_norm HBU).
-      apply: sss_compute_trans.
-      { apply: (subcode_sss_compute (P := (_, CASE_VAR0 _ _))).
-        { eexists _, _. rewrite /PROG. by do 3 rewrite [LHS]app_assoc. }
-        rewrite ?H'. apply: CASE_VAR0_spec.
-        do ? (rewrite vec_change_neq; first done). by eassumption. }
+      apply: (concat_sss_compute_trans 4).
+      { apply: CASE_VAR0_spec. do ? (rewrite vec_change_neq; first done). by eassumption. }
       apply: sss_compute_refl'. by rewrite (counters_eta v).
     + (* case (var (S n)) *)
       move=> ? ctx'' H1v H2v H3v  [<- <- <-].
@@ -855,19 +705,14 @@ Proof.
       split. { move: H2v. by rewrite (counters_eta v). }
       split. { move: H3v. by rewrite (counters_eta v). }
       apply: sss_progress_compute_trans.
-      { apply: (subcode_sss_progress (P := (_, NOOP _))).
-        { by eexists [], _. }
-        rewrite ?H'. by apply: NOOP_spec. }
-      apply: sss_compute_trans.
-      { apply: (subcode_sss_compute (P := (_, UNPACK _ _ _))).
-        { by eexists _, _. }
-        rewrite ?H'. by apply: (UNPACK_spec H3v). }
-      rewrite ?Nat.add_assoc. apply: mma_step. rewrite /= !(vec_norm HAB).
+      { apply: sss_compute_progress.
+        { by apply: (concat_sss_compute_trans 0); [apply JMP_spec | apply: sss_compute_refl]. }
+        case. rewrite /JMP_len /=. lia. }
+      apply: (concat_sss_compute_trans 1). { by apply: (UNPACK_spec H3v). }
+      rewrite /= ?Nat.add_assoc. apply: mma_step. rewrite /= !(vec_norm HAB).
       rewrite ?Nat.add_assoc. apply: mma_step. rewrite /= !(vec_norm HAU) !(vec_norm HBU).
-      apply: sss_compute_trans.
-      { apply: (subcode_sss_compute (P := (_, CASE_VARS _ _))).
-        { eexists _, _. rewrite /PROG. by do 4 rewrite [LHS]app_assoc. }
-        rewrite ?H'. apply: CASE_VARS_spec.
+      apply: (concat_sss_compute_trans 5).
+      { apply: CASE_VARS_spec.
         - do ? (rewrite vec_change_neq; first done). by eassumption.
         - by rewrite (vec_change_eq erefl).
         - do ? (rewrite vec_change_neq; first done). by rewrite (vec_change_eq erefl). }
@@ -879,19 +724,14 @@ Proof.
     split. { move: H2v. by rewrite (counters_eta v). }
     split. { move: H3v. by rewrite (counters_eta v). }
     apply: sss_progress_compute_trans.
-    { apply: (subcode_sss_progress (P := (_, NOOP _))).
-      { by eexists [], _. }
-      rewrite ?H'. by apply: NOOP_spec. }
-    apply: sss_compute_trans.
-    { apply: (subcode_sss_compute (P := (_, UNPACK _ _ _))).
-      { by eexists _, _. }
-      rewrite ?H'. by apply: (UNPACK_spec H3v). }
-    rewrite ?Nat.add_assoc. apply: mma_step. rewrite /= -/enc_term !(vec_norm HAB).
+    { apply: sss_compute_progress.
+      { by apply: (concat_sss_compute_trans 0); [apply JMP_spec | apply: sss_compute_refl]. }
+      case. rewrite /JMP_len /=. lia. }
+    apply: (concat_sss_compute_trans 1). { by apply: (UNPACK_spec H3v). }
+    rewrite /= ?Nat.add_assoc. apply: mma_step. rewrite /= -/enc_term !(vec_norm HAB).
     rewrite ?Nat.add_assoc. apply: mma_step. rewrite /= !(vec_norm HAB).
-    apply: sss_compute_trans.
-    { apply: (subcode_sss_compute (P := (_, CASE_APP _ _))).
-      { eexists _, _. rewrite /PROG. by do 7 rewrite [LHS]app_assoc. }
-      rewrite ?H'. apply: CASE_APP_spec.
+    apply: (concat_sss_compute_trans 8).
+    { apply: CASE_APP_spec.
       - do ? (rewrite vec_change_neq; first done). by eassumption.
       - do ? (rewrite vec_change_neq; first done). by eassumption.
       - do ? (rewrite vec_change_neq; first done). by rewrite (vec_change_eq erefl). }
@@ -904,26 +744,21 @@ Proof.
     split. { move: H2v. by rewrite (counters_eta v). }
     split. { move: H3v. by rewrite (counters_eta v). }
     apply: sss_progress_compute_trans.
-    { apply: (subcode_sss_progress (P := (_, NOOP _))).
-      { by eexists [], _. }
-      rewrite ?H'. by apply: NOOP_spec. }
-    apply: sss_compute_trans.
-    { apply: (subcode_sss_compute (P := (_, UNPACK _ _ _))).
-      { by eexists _, _. }
-      rewrite ?H'. by apply: (UNPACK_spec H3v). }
-    rewrite ?Nat.add_assoc. apply: mma_step. rewrite /= -/enc_term !(vec_norm HAB).
+    { apply: sss_compute_progress.
+      { by apply: (concat_sss_compute_trans 0); [apply JMP_spec | apply: sss_compute_refl]. }
+      case. rewrite /JMP_len /=. lia. }
+    apply: (concat_sss_compute_trans 1). { by apply: (UNPACK_spec H3v). }
+    rewrite /= ?Nat.add_assoc. apply: mma_step. rewrite /= -/enc_term !(vec_norm HAB).
     rewrite ?Nat.add_assoc. apply: mma_step. rewrite /= !(vec_norm HAB).
-    apply: sss_compute_trans.
-    { apply: (subcode_sss_compute (P := (_, CASE_LAM _ _))).
-      { eexists _, _. rewrite /PROG. by do 6 rewrite [LHS]app_assoc. }
-      rewrite ?H'. apply: CASE_LAM_spec.
+    apply: (concat_sss_compute_trans 7).
+    { apply: CASE_LAM_spec.
       - do ? (rewrite vec_change_neq; first done). by eassumption.
       - do ? (rewrite vec_change_neq; first done). by eassumption.
       - do ? (rewrite vec_change_neq; first done). by rewrite (vec_change_eq erefl). }
     apply: sss_compute_refl'. by rewrite (counters_eta v).
 Qed.
 
-Arguments Krivine_step : simpl never.
+#[local] Arguments Krivine_step : simpl never.
 
 Lemma simulation {ts ctx t} v : halt_cbn ts ctx t ->
   vec_pos v TS = enc_cs ts ->
@@ -936,20 +771,12 @@ Proof.
   { move=> v ts ctx t [] -> -> ->.
     rewrite /sss_terminates /sss_output.
     move=> H1v H2v H3v. eexists. split.
-    - apply: sss_compute_trans.
-      { apply: (subcode_sss_compute (P := (_, NOOP _))).
-        { by eexists [], _. }
-        apply: sss_progress_compute. by apply: NOOP_spec. }
-      apply: sss_compute_trans.
-      { apply: (subcode_sss_compute (P := (_, UNPACK _ _ _))).
-        { by eexists _, _. }
-        rewrite ?H'. by apply: (UNPACK_spec H3v). }
-      rewrite ?Nat.add_assoc. apply: mma_step. rewrite /= -/enc_term !(vec_norm HAB).
+    - apply: (concat_sss_compute_trans 0). { by apply: JMP_spec. }
+      apply: (concat_sss_compute_trans 1). { by apply: (UNPACK_spec H3v). }
+      rewrite /= ?Nat.add_assoc. apply: mma_step. rewrite /= -/enc_term !(vec_norm HAB).
       rewrite ?Nat.add_assoc. apply: mma_step. rewrite /= !(vec_norm HAB).
-      apply: sss_compute_trans.
-      { apply: (subcode_sss_compute (P := (_, CASE_LAM _ _))).
-        { eexists _, _. rewrite /PROG. by do 6 rewrite [LHS]app_assoc. }
-        rewrite ?H'. apply: CASE_LAM_spec'.
+      apply: (concat_sss_compute_trans 7).
+      { apply: CASE_LAM_spec'.
         do ? (rewrite vec_change_neq; first done). by eassumption. }
       apply: sss_compute_refl.
     - left. rewrite /=. lia. }
@@ -969,27 +796,6 @@ Require Import Undecidability.Shared.Libs.DLW.Code.subcode.
 
 #[local] Notation all := (fold_right and True).
 
-Fixpoint eclosed (u : eterm) :=
-  let '(closure ctx t) := u in bound (length ctx) t /\ all (map eclosed ctx).
-
-Lemma Krivine_step_eclosed ts ctx t ts' ctx' t' :
-  Krivine_step (ts, ctx, t) = Some (ts', ctx', t') ->
-  all (map eclosed ts) -> eclosed (closure ctx t) ->
-  all (map eclosed ts') /\ eclosed (closure ctx' t').
-Proof.
-  rewrite /Krivine_step. case: t.
-  - move=> [|n].
-    + case: ctx; first done.
-      move=> [? ?] ? [<- <- <-] /=. tauto.
-    + case: ctx; first done.
-      move=> [? ?] ? [<- <- <-] /= ? [/boundE ?] [[]] *.
-      split; [done|split;[|done]]. constructor. lia.
-  - move=> > [<- <- <-] /= ? [/boundE]. tauto.
-  - move=> ?. case: ts; first done.
-    move=> > [<- <- <-] /= ? [/boundE]. tauto.
-Qed.
-
-(* needs closedness of input so that there are no illegal inputs *)
 Lemma inverse_simulation ts ctx t v :
   vec_pos v TS = enc_cs ts ->
   vec_pos v CTX = enc_cs ctx ->
@@ -1038,17 +844,11 @@ Definition input t :=
 End Argument.
 
 Require Import Undecidability.Synthetic.Definitions.
-Require Import Undecidability.L.Util.L_facts.
-Require Import Undecidability.LambdaCalculus.Util.term_facts.
 
 Theorem reduction : KrivineMclosed_HALT ⪯ (@MMA_HALTING 5).
 Proof.
-  exists (fun '(exist _ t _) => 
-    (Argument.PROG 1, Argument.input t)).
-  move=> [t Ht]. split.
+  exists (fun '(exist _ t _) => (Argument.PROG 1, Argument.input t)).
+  move=> [t /= /eclosed_closed Ht]. split.
   - move=> /Argument.simulation. by apply.
-  - move=> /Argument.inverse_simulation. apply; [done..|].
-    split; last done.
-    apply /closed_dcl /closed_I.
-    move=> ?. by rewrite L_subst_wCBN_subst.
+  - move=> /Argument.inverse_simulation. by apply.
 Qed.
